\documentclass[../electromagnetism.tex]{subfiles}
\begin{document}
\section{Plane Harmonic Waves}
The wave equation in 4d is the following second order partial differential equation
\begin{equation}
	\pdv[2]{f}{x}+\pdv[2]{f}{y}+\pdv[2]{f}{z}=\frac{1}{u^2}\pdv[2]{f}{t}
	\label{eq:3dwaveeq}
\end{equation}
Taken the simpler case of a wave equation moving through a single spatial dimension, i.e.
\begin{equation*}
	\pdv[2]{f}{x}=\frac{1}{u^2}\pdv[2]{f}{t}
\end{equation*}
We already know that it has a simple solution in terms of cosines (or sines)
\begin{equation}
	f(x,t)=f_0\cos(kx-\omega t)
	\label{eq:1dwavesol}
\end{equation}
Given that
\begin{equation*}
	\frac{\omega}{k}=u
\end{equation*}
The solution \eqref{eq:1dwavesol} is of particular importance in treating electromagnetic waves (or waves in general). It tells us that the wave $f(x,t)$ varies sinusoidally with the distance $x$ and it's harmonic in $t$ for any given point in space.\\
Fixing the position and moving only through time, going to a new time $t+\Delta t$, we have that due to the previous constraint the point $x$ will have moved by $\Delta x=u\Delta t$.\\
It's exactly like adding a phase to the wave (hence the name \textit{phase velocity} of $u$). Note that if we used another solution, say
\begin{equation*}
	f_r(x,t)=f_0\cos(kx+\omega t)
\end{equation*}
We would describe a wave going back, with displacement $\Delta x=-u\Delta t$ for some given time.\\
In terms of electrodynamics, all these constants have names:
\begin{itemize}
\item $u$ is the phase velocity
\item $\lambda$ is the wavelength
\item $\omega$ is the angular frequency
\item $k$ is the angular wavenumber
\end{itemize}
There are also other derived values that have given name, which are
\begin{itemize}
\item $T$ the period, for which $\lambda=uT=\frac{2\pi}{k}$
\item $\nu$ the frequency, for which $\nu=\frac{u}{\lambda}=\frac{\omega}{2\pi}=T^{-1}$
\item $\sigma$ the spectroscopic wavenumber, for which $\sigma=\frac{1}{\lambda}$
\end{itemize}
Going back to waves in 3 spatial dimensions, the general solution of the wave equation \eqref{eq:3dwaveeq} is known as a \textit{plane harmonic wave}, and has the following mathematical shape
\begin{equation}
	f(x,y,z,t)=f_0\cos\left( k^ix_i-\omega t \right)
	\label{eq:3dwavesol}
\end{equation}
Here the angular wavenumber (or wavenumber for simplicity), is a vector, and is known as the \textit{propagation vector} $k^i$. The magnitude of this vector \emph{is the actual wavenumber}, i.e.
\begin{equation*}
	k=\sqrt{k^ik_i}
\end{equation*}
The physical meaning of this solution resides mostly inside the cosine argument, $k^ix_i-\omega t$.\\
Setting it as constant we get the equation of a plane in space, which are called the \textit{surfaces of constant phase}. The normals of these surfaces (planes) are proportional and perpendicular to the wavevector, and these planes ``move'' in that direction at a rate equal to the phase velocity $u$
\subsection{Alternative Representations of the Wavefunction}
We can think immediately about alternative representations of the wavefunction \eqref{eq:3dwavesol}. One of these is by using the definition of the constant phase surfaces we gave before, in fact, as we said $k^i=k\hat{n}^i$, and therefore
\begin{equation*}
	f(x^i,t)=f_0\cos\left[ (x^i\hat{n}_i-ut)k \right]
\end{equation*}
Remember that $ku=\omega$.\\
Another one, is by using complex functions. Using the Euler identity for the complex exponential we can write
\begin{equation*}
	f(x^i,t)=F_0e^{i\left( k^ix_i-\omega t \right)}
\end{equation*}
Note that since generally $F_0\in\Cf$, the actual physical quantity is the real part of $f$.\\
One use of the complex wavefunction is immediate when dealing with spherical waves, where $x^i=r$ and
\begin{equation}
	f(r,t)=\frac{1}{r}\cos(kr-\omega t)=\real\left\{ \frac{1}{r}e^{i(kr-\omega t)} \right\}
	\label{eq:sphericaleq}
\end{equation}
Ignoring the real part on the right it's clear that the second will be extremely easier to manipulate.
\section{Group Velocity}
Suppose now that we have two harmonic waves $\phi,\psi$ with different angular frequencies $\omega_1=\omega+\Delta\omega$ and $\omega_2=\omega-\Delta\omega$.\\
In general also the wavenumbers will differ, and we'll call them for simplicity $k_1=k+\Delta k$, $k_2=k-\Delta k$. Supposing that the waves have the same amplitude $A$ and are traveling in the same direction (say z), the superposition of the two will be
\begin{equation*}
	\Psi=\psi+\phi=A\left( e^{i\left( (k+\Delta k)z-(\omega+\Delta\omega)t \right)}+e^{i\left( (k-\Delta k)z-(\omega-\Delta\omega)t \right)} \right)
\end{equation*}
Collecting terms 
\begin{equation*}
	\Psi=Ae^{i\left( kz-\omega t \right)}\left( e^{i\left( z\Delta k-t\Delta\omega \right)}+e^{-i\left( z\Delta k-t\Delta\omega \right)} \right)
\end{equation*}
Recognizing a $2\cos(\cdots)$ on the right we have that
\begin{equation*}
	\Psi=2Ae^{i\left( kz-\omega t \right)}\cos\left( z\Delta k-t\Delta\omega \right)
\end{equation*}
The result of this superposition is a new wave $\eta$, with amplitude $B=2A$ multiplied by a ``modulation envelope'' given by the cosine.\\
From the previous results it's clear that this envelope doesn't travel at the phase velocity, in fact, we have a new propagation velocity, known as the \textit{group velocity}
\begin{equation}
	u_g=\frac{\Delta\omega}{\Delta k}
	\label{eq:groupvelwaves}
\end{equation}
At the limit, we have that $\omega'(k)=u_g$, and since $\omega=ku$ or $\omega=kc/n$ we have
\begin{equation*}
	u_g=\dv{k}\left( \frac{kc}{n} \right)=\frac{c}{n}-\frac{ck}{n^2}\dv{n}{k}=u\left( 1-\frac{k}{n}\dv{n}{k} \right)
\end{equation*}
Note that we wrote $n=n(k)$! The refraction index is in general dependent on the angular frequency $\omega$, and therefore on $k$! As an example, you can see how different wavelengths of light behave passing through glass. They go through when $\lambda$ is in the range of visible light, but are completely opaque in infrared, i.e. $n$ \emph{must} vary with frequency (or wavelength, or wavenumber, or \ldots)\\
From the previous monologue and from the definitions we can then say that
\begin{equation}
	\begin{aligned}
		u_g&=u\left( 1-\frac{k}{n}\dv{n}{k} \right)\\
		u_g&=u-\lambda\dv{u}{\lambda}\\
		\frac{1}{u_g}&=\frac{1}{u}-\frac{\lambda_0}{c}\dv{n}{\lambda_0}
	\end{aligned}
	\label{eq:groupvelder}
\end{equation}
Where $\lambda_0$ is the vacuum wavelength.\\
Phase velocity and group velocity can only be equal in vacuum ($n=0$), where $u_g=u=c$.
%%TODO DOPPLER EFFECT
\begin{comment}
\section{Doppler Effect}
Consider a source of waves and an observer moving in relative motion from one another. The frequency observed is changed compared to the measured frequency when there is no relative motion.\\
Say that the source is moving away from the receiver with velocity $u$. It's observed that the measured frequency is expanded from $\nu$ to $c+\nu$ with $c$ being the speed of the waves.\\
The observed frequency is
\begin{equation}
	\nu'=\nu\left( \frac{c}{c+u} \right)\approx\nu\left( 1-\frac{u}{c}+\frac{u^2}{c^2} \right)
	\label{eq:awayfreqdoppler}
\end{equation}
While, if the receiver (or the source) is moving away from the receiver, we will have
\begin{equation}
	\nu'=\nu\left( \frac{c-u}{c} \right)=\nu\left( 1-\frac{u}{c} \right)
	\label{eq:closerdoppler}
\end{equation}
or
\begin{equation*}
	\frac{\Delta\nu}{\nu}=\frac{u}{c}
\end{equation*}
These formulas, with these considerations, although equal to the first order, make no sense in the context of special relativity. The measured frequency is instead
\begin{equation}
	\nu'=n\sqrt{\frac{1-u/c}{1+u/c}}\approx\nu\left( 1-\frac{u}{c}+\frac{1}{2}\frac{u^2}{c^2} \right)
	\label{eq:reldoppler}
\end{equation}
Notice how the first order of the relativistic formula is exactly the same of the classical case
\end{comment}
\end{document}
